#+BEGIN_SRC python :session :results output
def add(p1, p2, curve, p):
    """blah"""
    if p1 is None:
        return p2
    if p2 is None:
        return p1
    if (p1[0] == p2[0]) and (p1[1] == -(p2[1])):
        return None
    lam = 0
    if p1 == p2:
        lam = ((3*(p1[0]**2)+curve[0])*inverse_modp(2*p1[1], p)) % p
    else:
        lam = ((p2[1] - p1[1])*inverse_modp(p2[0] - p1[0], p)) % p
    x3 = (lam**2 - p1[0] - p2[0]) % p
    y3 = (lam*(p1[0] - x3) - p1[1]) % p
    return x3, y3
# Denote the point at infinity by 'None'
# a curve is represented by a 2-tuple (a, b)
# for y^2 = x^3 + ax + b
#+END_SRC

#+RESULTS:

#+BEGIN_SRC python :session :results output
#try example
curve = (3, 8)
p = (9, 7)
q = (1, 8)
add(p, q, curve, 13) # (2, 10)



#+END_SRC

#+RESULTS:
: 
: >>> >>> >>> (2, 10)

#+BEGIN_SRC python :session

#+END_SRC
